Library compiles.

lib/Array.v
@@ -16,29 +16,20 @@ Parameter array : Type -> Type.
 
 Parameter length : forall T, array T -> nat.
 
-Instance bagCard T : BagCard (array T) := {|
-    card := @length T
-  |}.
+Parameter read_option : forall T, array T -> nat -> option T.
 
-Parameter bagReadOption : forall T, BagReadOption nat T (array T).
-Instance _bagReadOption : forall T, BagReadOption nat T (array T) := bagReadOption. (* FIXME: Some mechanism to avoid this repeation? *)
-Instance bagRead T `{Inhab T} : BagRead nat T (array T) :=
-  ReadOptionToRead nat T (array T).
+Parameter write : forall T, array T -> nat -> T -> array T.
 
-Parameter bagUpdate : forall T, BagUpdate nat T (array T).
-Instance _bagUpdate : forall T, BagUpdate nat T (array T) := bagUpdate.
-Definition write {T} : array T -> nat -> T -> array T :=
-  LibContainer.update.
+Parameter empty : forall T, array T.
 
-Parameter bagEmpty : forall T, BagEmpty (array T).
-Instance _bagEmpty : forall T, BagEmpty (array T) := bagEmpty.
+Parameter map : forall T1 T2, (T1 -> T2) -> array T1 -> array T2.
 
 Parameter from_list : forall T, list T -> array T.
 Parameter to_list : forall T, array T -> list T.
 
-Parameter read_option_Some : forall T `{Inhab T} (a : array T) n,
+Parameter read_option_Some_exists : forall T (a : array T) n,
   n < length a ->
-  read_option a n = Some (read a n).
+  exists v, read_option a n = Some v.
 
 Parameter read_option_None : forall T (a : array T) n,
   n >= length a ->
@@ -53,20 +44,11 @@ Parameter read_option_write_neq : forall T a (t : T) n1 n2,
   n1 <> n2 ->
   read_option (write a n1 t) n2 = read_option a n2.
 
-Parameter read_write_eq : forall T `{Inhab T} a (t : T) n,
-  n < length a ->
-  read (write a n t) n = t.
-
-Parameter read_write_neq : forall T `{Inhab T} a (t : T) n1 n2,
-  n2 < length a ->
-  n1 <> n2 ->
-  read (write a n1 t) n2 = read a n2.
-
 Parameter write_length : forall T a (t : T) n,
   length (write a n t) = length a.
 
 Parameter empty_length : forall T,
-  length (empty : array T) = 0.
+  length (@empty T) = 0.
 
 Parameter from_list_length : forall T (l : list T),
   length (from_list l) = LibList.length l.
@@ -80,69 +62,124 @@ Parameter from_list_read_option : forall T (l : list T) n,
 Parameter to_list_read_option : forall T (a : array T) n,
   nth_option n (to_list a) = read_option a n.
 
-Parameter from_list_read : forall T `{Inhab T} (l : list T) n,
-  read (from_list l) n = nth n l.
+Parameter map_length : forall T1 T2 (f : T1 -> T2) a,
+  length (map f a) = length a.
 
-Parameter to_list_read : forall T `{Inhab T} (a : array T) n,
-  nth n (to_list a) = read a n.
+Parameter map_read_option : forall T1 T2 (f : T1 -> T2) a n v,
+  read_option a n = Some v ->
+  read_option (map f a) n = Some (f v).
 
 End ArraySpec.
 
 
-Module Type ArrayExtra (A : ArraySpec).
+Module ArrayExtra (A : ArraySpec).
 
-Import A.
-
-Parameter map : forall T1 T2, (T1 -> T2) -> array T1 -> array T2.
-
-Parameter map_length : forall T1 T2 (f : T1 -> T2) a,
-  length (map f a) = length a.
-
-Parameter map_read : forall T1 T2 `{Inhab T1} `{Inhab T2} (f : T1 -> T2) a n,
-  n < length a ->
-  read (map f a) n = f (read a n).
-
-End ArrayExtra.
-
-
-(** * Implementation **)
-
-Module ArrayList <: ArraySpec.
-
-Definition array := list.
-
-Definition length : forall T, array T -> nat := length.
+Include A.
 
 Instance bagCard T : BagCard (array T) := {|
     card := @length T
   |}.
 
 Instance bagReadOption T : BagReadOption nat T (array T) := {|
-    read_option a n := nth_option n a
+    Heap.read_option := @read_option T
   |}.
-Instance _bagReadOption : forall T, BagReadOption nat T (array T) := bagReadOption.
 Instance bagRead T `{Inhab T} : BagRead nat T (array T) :=
   ReadOptionToRead nat T (array T).
 
 Instance bagUpdate T : BagUpdate nat T (array T) := {|
-    LibContainer.update a n t := update n t a
+    LibContainer.update a n t := write a n t
   |}.
-Instance _bagUpdate : forall T, BagUpdate nat T (array T) := bagUpdate.
-Definition write {T} : array T -> nat -> T -> array T :=
-  LibContainer.update.
-
-Definition from_list T := id : list T -> array T.
-Definition to_list T := id : array T -> list T.
 
 Instance bagEmpty T : BagEmpty (array T) := {|
-   empty := from_list nil
+   LibContainer.empty := empty T
  |}.
-Instance _bagEmpty : forall T, BagEmpty (array T) := bagEmpty.
 
 Lemma read_option_Some : forall T `{Inhab T} (a : array T) n,
   n < length a ->
   read_option a n = Some (read a n).
-Proof. introv I. simpl. erewrite~ @nth_option_Some. Qed.
+Proof.
+  introv I. forwards~ (v&E): read_option_Some_exists I.
+  simpl. rewrite~ E.
+Qed.
+
+Lemma None_read_option : forall T (a : array T) n,
+  read_option a n = None ->
+  n >= length a.
+Proof.
+  introv E. tests~: (n >= length a).
+  forwards (v&Ev): read_option_Some_exists a n. { nat_math. }
+  rewrite Ev in E. inverts E.
+Qed.
+
+Lemma read_write_eq : forall T `{Inhab T} a (t : T) n,
+  n < length a ->
+  read (write a n t) n = t.
+Proof. introv I. unfold write. simpl. rewrite~ read_option_write_eq. Qed.
+
+Lemma read_write_neq : forall T `{Inhab T} a (t : T) n1 n2,
+  n2 < length a ->
+  n1 <> n2 ->
+  read (write a n1 t) n2 = read a n2.
+Proof. introv I D. unfold write. simpl. rewrite~ read_option_write_neq. Qed.
+
+Lemma from_list_read : forall T `{Inhab T} (l : list T) n,
+  n < LibList.length l ->
+  read (from_list l) n = nth n l.
+Proof.
+  introv I. lets E: (from_list_read_option l n).
+  rewrite read_option_Some with (H := H) in E.
+  - symmetry in E. apply nth_option_defined with (H := H) in E. rewrite~ <- E.
+  - rewrite~ from_list_length.
+Qed.
+
+Lemma to_list_read : forall T `{Inhab T} (a : array T) n,
+  n < length a ->
+  nth n (to_list a) = read a n.
+Proof.
+  introv I. lets E: (to_list_read_option a n).
+  rewrite read_option_Some with (H := H) in E; autos~.
+  apply nth_option_defined with (H := H) in E; autos~.
+Qed.
+
+Lemma map_read : forall T1 T2 `{Inhab T1} `{Inhab T2} (f : T1 -> T2) a n,
+  n < length a ->
+  read (map f a) n = f (read a n).
+Proof.
+  introv I. forwards E1: read_option_Some I. forwards E2: map_read_option f E1.
+  rewrite <- (map_length f) in I. forwards E3: read_option_Some I.
+  rewrite E3 in E2. inverts~ E2.
+Qed.
+
+End ArrayExtra.
+
+
+(** * Implementation **)
+
+Module ArrayList : ArraySpec.
+
+Definition array T := list T.
+
+Definition length : forall T, array T -> nat := length.
+
+Definition read_option T (a : array T) n := nth_option n a.
+
+Definition write {T} (a : array T) n t := update n t a.
+
+Definition from_list T := id : list T -> array T.
+Definition to_list T := id : array T -> list T.
+
+Definition empty T : array T := nil.
+
+Definition map : forall T1 T2, (T1 -> T2) -> array T1 -> array T2 := LibList.map.
+
+Lemma read_option_Some_exists : forall T (a : array T) n,
+  n < length a ->
+  exists v, read_option a n = Some v.
+Proof.
+  introv I. destruct read_option eqn: E.
+  - autos*.
+  - unfolds in E. apply nth_option_length in E. unfolds length. nat_math.
+Qed.
 
 Lemma read_option_None : forall T (a : array T) n,
   n >= length a ->
@@ -164,21 +201,6 @@ Proof.
   - fequals. unfold write. apply~ update_out. unfolds length. nat_math.
 Qed.
 
-Lemma read_write_eq : forall T `{Inhab T} a (t : T) n,
-  n < length a ->
-  read (write a n t) n = t.
-Proof. introv I. unfold write. simpl. rewrite~ nth_option_update_eq. Qed.
-
-Lemma read_write_neq : forall T `{Inhab T} a (t : T) n1 n2,
-  n2 < length a ->
-  n1 <> n2 ->
-  read (write a n1 t) n2 = read a n2.
-Proof.
-  introv I D. unfold write. simpl. tests I': (n1 < length a).
-  - rewrite~ nth_option_update_neq.
-  - rewrite~ update_ge_length. unfolds length. nat_math.
-Qed.
-
 Lemma write_length : forall T a (t : T) n,
   length (write a n t) = length a.
 Proof. introv. apply~ length_update. Qed.
@@ -192,7 +214,7 @@ Lemma to_list_length : forall T (a : array T),
 Proof. reflexivity. Qed.
 
 Lemma empty_length : forall T,
-  length (empty : array T) = 0.
+  length (empty T) = 0.
 Proof. reflexivity. Qed.
 
 Lemma from_list_read_option : forall T (l : list T) n,
@@ -203,43 +225,17 @@ Lemma to_list_read_option : forall T (a : array T) n,
   nth_option n (to_list a) = read_option a n.
 Proof. reflexivity. Qed.
 
-Lemma from_list_read : forall T `{Inhab T} (l : list T) n,
-  read (from_list l) n = nth n l.
-Proof.
-  introv. simpl. destruct nth_option eqn: E.
-  - forwards*: nth_option_defined E.
-  - symmetry. apply nth_option_length in E.
-    forwards A: nth_default_gt_length; [ apply~ E | apply~ A ].
-Qed.
-
-Lemma to_list_read : forall T `{Inhab T} (a : array T) n,
-  nth n (to_list a) = read a n.
-Proof. introv. symmetry. apply~ from_list_read. Qed.
-
-End ArrayList.
-
-
-Module ArrayListExtra <: ArrayExtra (ArrayList).
-
-Include ArrayList.
-
-Definition map : forall T1 T2, (T1 -> T2) -> array T1 -> array T2 := LibList.map.
-
 Lemma map_length : forall T1 T2 (f : T1 -> T2) a,
   length (map f a) = length a.
 Proof. introv. apply~ length_map. Qed.
 
-Lemma map_read : forall T1 T2 `{Inhab T1} `{Inhab T2} (f : T1 -> T2) a n,
-  n < length a ->
-  read (map f a) n = f (read a n).
-Proof.
-  introv I. simpl. destruct nth_option eqn:E1.
-  - forwards E1': nth_option_defined E1. destruct (nth_option n a) eqn:E2.
-    + forwards E2': nth_option_defined E2. substs~. apply~ map_nth.
-    + apply nth_option_length in E2. erewrite <- map_length in E2.
-      apply nth_option_length in E2. rewrite E1 in E2. false~ E2.
-  - apply nth_option_length in E1. erewrite map_length in E1. false. nat_math.
-Qed.
+Lemma map_read_option : forall T1 T2 (f : T1 -> T2) a n v,
+  read_option a n = Some v ->
+  read_option (map f a) n = Some (f v).
+Proof. introv E. apply Nth_nth_option in E. apply Nth_nth_option. applys~ map_Nth E. Qed.
 
-End ArrayListExtra.
+End ArrayList.
+
+
+Module ArrayListExtra := ArrayExtra (ArrayList).
 
